\documentclass[a4paper]{article}

\usepackage[english]{babel}
\usepackage[utf8]{inputenc}
\usepackage{amsmath}
\usepackage{graphicx}
\usepackage[colorinlistoftodos]{todonotes}
\usepackage[margin=0.5in]{geometry}

\title{5/15 Lecture}
\author{David Behrle}
 
\begin{document}
\date{May 15, 2024}
\maketitle
    \section{Dot products}
    \subsection{equations}
        \begin{equation}
            \vec{A} \cdot \vec{B} = s
        \end{equation}

        \begin{equation}
            \vec{A} \cdot \vec{B} = |A||B|cos(\theta)
        \end{equation}

        \begin{equation}
            \vec{A} \cdot \vec{B} = A_{\parallel}B = AB_{\parallel} = ABcos(\theta)
        \end{equation}

        \begin{equation}
            \vec{A} = A_x\hat{i} + A_y\hat{j} + A_z\hat{k} = (A_x, A_y, A_z)
        \end{equation}

        \begin{equation}
            \vec{B} = B_x\hat{i} + B_y\hat{j} + B_z\hat{k} = (B_x, B_y, B_z)
        \end{equation}

        \begin{equation}
            s = \vec{A} \cdot \vec{B} = A_xB_x + A_yB_y + A_zB_z
        \end{equation}
    \subsection{i, j, k components}
        \begin{equation}
            \hat{i} \cdot \hat{i} = (\hat{i})^2 = 1
        \end{equation}

        \begin{equation}
            \hat{j} \cdot \hat{j} = (\hat{j})^2 = 1
        \end{equation}

        \begin{equation}
            \hat{k} \cdot \hat{k} = (\hat{k})^2 = 1
        \end{equation}

        \begin{equation}
            \hat{i} \cdot \hat{j} = 0
        \end{equation}

        \begin{equation}
            \hat{i} \cdot \hat{k} = 0
        \end{equation}

    \section{Cross products}
    \subsection{equations}
        \begin{equation}
            \hat{i} \times \hat{j} = \hat{k}
        \end{equation}

        \begin{equation}
            \hat{j} \times \hat{k} = \hat{i}
        \end{equation}

        \begin{equation}
            \hat{k} \times \hat{i} = \hat{j}
        \end{equation}

        order matters
        \begin{equation}
            \vec{A} \times \vec{B} \neq \vec{B} \times \vec{A}
        \end{equation}

        \begin{equation}
            \hat{k} \times \hat{i} = \hat{j} 
        \end{equation}

        \begin{equation}
            \hat{i} \times \hat{k} = -\hat{j}
        \end{equation}

\end{document}